little fixes in IFC with Catalin, going to the style of the paper

examples/dm4free/FStar.DM4F.IFC.fst
@@ -10,27 +10,20 @@ type label =
   | High
 *)
 type label = bool
-inline let low = true
-inline let high = false
+let low = true
+let high = false
 
-(* working around the whitelist *)
-inline let eq l1 l2 =
-  match l1, l2 with
-  | true, true
-  | false, false -> true
-  | _, _ -> false
+let join l1 l2 =
+    if l1 = high || l2 = high then high else low
 
-inline let join l1 l2 =
-  if l1 `eq` high || l2 `eq` high then high else low
-
-inline let flows l1 l2 = not(l1 `eq` high && l2 `eq` low)
+let flows l1 l2 = not(l1=high && l2=low)
 
 let ifc (a:Type) = label -> M (option (a * label))
 
 (* open FStar.FunctionalExtensionality *)
 
-let eq_ifc (a:Type) (f:ifc a) (g:ifc a) =
-   forall l. f l == g l
+(* let eq_ifc (a:Type) (f:ifc a) (g:ifc a) = *)
+(*    forall l. f l == g l *)
 
 let return_ifc (a:Type) (x:a) : ifc a = fun l -> Some (x, l)
 let bind_ifc (a:Type) (b:Type) (f:ifc a) (g: a -> Tot (ifc b)) : ifc b
@@ -41,59 +34,42 @@ let bind_ifc (a:Type) (b:Type) (f:ifc a) (g: a -> Tot (ifc b)) : ifc b
              | None -> None
              | Some (y, l2) -> Some(y, l2)
 
-val left_unit: a:Type -> b:Type -> x:a -> f:(a -> Tot (ifc b))
-            -> Lemma (eq_ifc b (bind_ifc a b (return_ifc a x) f) (f x))
-let left_unit a b x f = admit() (* #710 *)
+(* val left_unit: a:Type -> b:Type -> x:a -> f:(a -> Tot (ifc b)) *)
+(*             -> Lemma (eq_ifc b (bind_ifc a b (return_ifc a x) f) (f x)) *)
+(* let left_unit a b x f = admit() (\* #710 *\) *)
 
-val right_unit: a:Type -> f:ifc a -> Lemma (eq_ifc a (bind_ifc a a f (return_ifc a)) f)
-let right_unit a f = admit() (* #710 *)
+(* val right_unit: a:Type -> f:ifc a -> Lemma (eq_ifc a (bind_ifc a a f (return_ifc a)) f) *)
+(* let right_unit a f = admit() (\* #710 *\) *)
 
-val associativity: a:Type -> b:Type -> c:Type -> f:ifc a -> g:(a -> Tot (ifc b)) -> h:(b -> Tot (ifc c))
-                 -> Lemma (eq_ifc c (bind_ifc a c f (fun x -> bind_ifc b c (g x) h)) (bind_ifc b c (bind_ifc a b f g) h))
-let associativity a b c f g h = ()
+(* val associativity: a:Type -> b:Type -> c:Type -> f:ifc a -> g:(a -> Tot (ifc b)) -> h:(b -> Tot (ifc c)) *)
+(*                  -> Lemma (eq_ifc c (bind_ifc a c f (fun x -> bind_ifc b c (g x) h)) (bind_ifc b c (bind_ifc a b f g) h)) *)
+(* let associativity a b c f g h = () *)
 
-// Some dummy implementations of actions for illustration purposes
-// Probably better to just take them axiomatically
-let read (l:label) : ifc bool =
-  (* fun l0 -> Some (true, join l0 l) -- needed to manually inline this; #711 *)
-  fun l0 -> match l0, l with
-            | low, low -> Some (true, low)
-            | _, _ -> Some (true, high)
 
-let write (l:label) (b:bool) : ifc unit =
-  (* fun l0 -> if flows l0 l then (Some ((), l0)) else None
-     -- needed to manually inline this; #711 *)
-  fun l0 -> match l0, l with
-            | high, low -> None
-            | _, _ -> Some ((), l0)
 
-let xor (b1:bool) (b2:bool) : Tot bool = not (b1 = b2)
-
-// A sample monadic program (normally would write this after
-// elaboration, but whatever, can write this in DM too)
-val p : unit -> Pure (ifc unit) (requires True) (ensures (fun r -> forall l. r l = None))
-(* Weak type (works): unit -> Tot (ifc unit) *)
-(* Alternative strong type (doesn't work), (Valid(ApplyTT@2 @0))
-  unit -> Tot (label -> Pure (err (unit * label)) (requires True) (ensures (fun r -> r = None))) *)
-(* let p () = bind_ifc _ _ (read low)              (fun b1 -> *)
-(*            bind_ifc _ _ (read low)              (fun b2 -> *)
-(*            bind_ifc _ _ (write low (b1 && b2))  (fun _  -> *)
-(*            bind_ifc _ _ (read high)             (fun b3 -> *)
-(*            bind_ifc _ _ (write high (b1 || b3)) (fun _  -> *)
-(*                         (write low (xor b3 b3))  ))))) *)
-let p () = admit() (* #710 *)
+(* // A sample monadic program (normally would write this after *)
+(* // elaboration, but whatever, can write this in DM too) *)
+(* val p : unit -> Pure (ifc unit) (requires True) (ensures (fun r -> forall l. r l = None)) *)
+(* (\* Weak type (works): unit -> Tot (ifc unit) *\) *)
+(* (\* Alternative strong type (doesn't work), (Valid(ApplyTT@2 @0)) *)
+(*   unit -> Tot (label -> Pure (err (unit * label)) (requires True) (ensures (fun r -> r = None))) *\) *)
+(* (\* let p () = bind_ifc _ _ (read low)              (fun b1 -> *\) *)
+(* (\*            bind_ifc _ _ (read low)              (fun b2 -> *\) *)
+(* (\*            bind_ifc _ _ (write low (b1 && b2))  (fun _  -> *\) *)
+(* (\*            bind_ifc _ _ (read high)             (fun b3 -> *\) *)
+(* (\*            bind_ifc _ _ (write high (b1 || b3)) (fun _  -> *\) *)
+(* (\*                         (write low (xor b3 b3))  ))))) *\) *)
+(* let p () = admit() (\* #710 *\) *)
 
 (* TODO: without reifiable, this fails weirdly. Cf #709 *)
 
+//#set-options "--debug FStar.DM4F.IFC --debug_level ED --debug_level Extreme --print_implicits --print_bound_var_types --log_queries"
 reifiable new_effect_for_free {
   IFC : a:Type -> Effect
   with
        repr         = ifc
      ; bind         = bind_ifc
      ; return       = return_ifc
-  and effect_actions
-      read = read
-    ; write = write
 }
 
 effect Ifc (a:Type) (req:IFC.pre) (ens:label -> option (a * label) -> GTot Type0) =
@@ -104,23 +80,27 @@ inline let lift_pure_exnst (a:Type) (wp:pure_wp a) (h0:label) (p:IFC.post a) =
   wp (fun a -> p (Some (a, h0)))
 sub_effect PURE ~> IFC = lift_pure_exnst
 
+assume val read : l:label -> IFC bool (fun l0 p -> forall b. p (Some (b, join l0 l)))
+assume val write : l:label -> bool -> IFC unit (fun l0 p -> if flows l0 l then p (Some ((), l0)) else  p None)
+let xor (b1:bool) (b2:bool) : Tot bool = not (b1 = b2)
+
 val p' : unit ->  Ifc unit (requires (fun l   -> True))
-                           (ensures  (fun l r -> r = None))
+                          (ensures  (fun l r -> r = None))
 let p' () =
-  let b1 = IFC.read low in
-  let b2 = IFC.read low in
-  IFC.write low (b1 && b2);
-  let b3 = IFC.read high in
-  IFC.write high (b1 || b3);
-  IFC.write low (xor b3 b3)
+  let b1 = read low in
+  let b2 = read low in
+  write low (b1 && b2);
+  let b3 = read high in
+  write high (b1 || b3);
+  write low (xor b3 b3)
 
-(* just a sanity check for Guido: this works with the pure to Ifc coercion;
-   btw. can't we get the pure to X coercion for free too ?*)
-val p'' : unit -> Ifc unit (requires (fun l   -> True))
-                           (ensures  (fun l r -> True))
-let p'' () = ()
+(* (\* just a sanity check for Guido: this works with the pure to Ifc coercion; *)
+(*    btw. can't we get the pure to X coercion for free too ?*\) *)
+(* val p'' : unit -> Ifc unit (requires (fun l   -> True)) *)
+(*                            (ensures  (fun l r -> True)) *)
+(* let p'' () = () *)
 
-(* [8:14:57 PM] Nik Swamy: I think for bonus points, in the ifc monad we could *)
-(* [8:15:33 PM] Nik Swamy: 1. add outputs, a list of Booleans, e.g., and have the write cons to it *)
-(* [8:15:48 PM] Nik Swamy: 2. add an input state so that read is not a constant *)
-(* [8:16:23 PM] Nik Swamy: 3. do a relational proof of the p program showing that despite the exception, the outputs would be the same in 2 runs *)
+(* (\* [8:14:57 PM] Nik Swamy: I think for bonus points, in the ifc monad we could *\) *)
+(* (\* [8:15:33 PM] Nik Swamy: 1. add outputs, a list of Booleans, e.g., and have the write cons to it *\) *)
+(* (\* [8:15:48 PM] Nik Swamy: 2. add an input state so that read is not a constant *\) *)
+(* (\* [8:16:23 PM] Nik Swamy: 3. do a relational proof of the p program showing that despite the exception, the outputs would be the same in 2 runs *\) *)
